\section{Basic Rules}
  \begin{enumerate}
    \item $\int x^n dx = \frac{x^{n+1}}{n+1} + c$
    \item $\int dx = x + c$
    \item $\int \frac{1}{\sqrt{x}} dx = 2\sqrt{x} + c$
    \item $\int \frac{1}{x^2} dx = -\frac{1}{x} + c$
    \item $\int 0 dx = c$ 
    \item $\int e^x dx = e^x + c$
    \item $\int a^x dx = \frac{a^x}{\ln a} + c$
    \item $\int \frac{1}{x} dx = \ln |x| + c$
    \item $\int \cos(x) dx = \sin(x) + c$
    \item $\int \sin(x) dx = -\cos(x) + c$
    \item $\int \sec^2(x) dx = \tan(x) + c$
    \item $\int \csc^2(x) dx = -\cot(x) + c$
    \item $\int \sec(x)\tan(x) dx = \sec(x) + c$
    \item $\int \csc(x)\cot(x) dx = -\csc(x) + c$
    \item $\int \frac{1}{\sqrt{1-x^2}} dx = \arcsin(x) + c = -\arccos(x) + c$
    \item $\int \frac{1}{1+x^2} dx = \arctan(x) + c = -\text{arccot}(x) + c$
    \item $\int \frac{1}{x\sqrt{x^2-1}} dx = \text{arcsec}(x) + c = -\text{arccsc}(x) + c$
  \end{enumerate}
